update

Test/civl/paxos/Paxos.bpl
@@ -23,13 +23,11 @@ datatype JoinResponse {
   JoinAccept(from: Node, lastVoteRound: int, lastVoteValue: Value),
   JoinReject(from: Node)
 }
-type JoinResponseChannel = Map Permission JoinResponse;
 
 datatype VoteResponse {
   VoteAccept(from: Node),
   VoteReject(from: Node)
 }
-type VoteResponseChannel = Map Permission VoteResponse;
 
 datatype Permission {
   JoinPerm(r:Round, n: Node),
@@ -111,8 +109,8 @@ var {:layer 0,1} joinChannel: [Round][JoinResponse]int;
 var {:layer 0,1} voteChannel: [Round][VoteResponse]int;
 
 // Intermediate channel representation
-var {:layer 1,1} {:linear} permJoinChannel: JoinResponseChannel;
-var {:layer 1,1} {:linear} permVoteChannel: VoteResponseChannel;
+var {:layer 1,1} {:linear} joinChannelPermissions: Set Permission;
+var {:layer 1,1} {:linear} voteChannelPermissions: Set Permission;
 var {:layer 1,1} {:linear} usedPermissions: Set Permission;
 
 ////////////////////////////////////////////////////////////////////////////////
@@ -128,12 +126,12 @@ function {:inline} InitLow (
   acceptorState: [Node]AcceptorState,
   joinChannel: [Round][JoinResponse]int,
   voteChannel: [Round][VoteResponse]int,
-  permJoinChannel: JoinResponseChannel,
-  permVoteChannel: VoteResponseChannel) : bool
+  joinChannelPermissions: Set Permission,
+  voteChannelPermissions: Set Permission) : bool
 {
   (forall n: Node :: acceptorState[n]->lastJoinRound == 0 && acceptorState[n]->lastVoteRound == 0) &&
   (forall r: Round, jr: JoinResponse :: joinChannel[r][jr] == 0) &&
   (forall r: Round, vr: VoteResponse :: voteChannel[r][vr] == 0) &&
-  permJoinChannel == Map_Empty() &&
-  permVoteChannel == Map_Empty()
+  joinChannelPermissions == Set_Empty() &&
+  voteChannelPermissions == Set_Empty()
 }
